\section{Full proof for theorem 1}

We need three lemmas as in \cite{jaakkola1993convergence}.

\begin{lemma}[Lemma 1 of \cite{jaakkola1993convergence}]
A random process 
$$
w_{n+1}(x) = (1-\alpha_n(x))w_n(x)+\beta_n(x)r_n(x)
$$
converges to zero with probability one if the following conditions are satisfied:
\begin{enumerate}
    \item $\sum_{n=1}^\infty \alpha_n(x) = \infty, \sum_{n=1}^\infty \alpha_n^2(x)<\infty$ and $\sum_{n=1}^\infty \beta_n(x) = \infty$, and $\sum_{n=1}^\infty \beta_n^2(x)<\infty$ uniformly over $x$ with probability one.
    \item $\mathbb{E}(r_n(x)|P_n,\beta_n) = 0$ and $\mathbb{E}(r_n^2(x)|P_n,\beta_n)\le C$ with probability one where
\end{enumerate}
    
\end{lemma}